src/Comp.v
@@ -1,0 +1,377 @@
+Require Export
+  Hask.Control.Monad.
+
+Require Import
+  Fiat.ADT
+  Fiat.ADTNotation.
+
+Program Instance Comp_Functor : Functor Comp := {
+  fmap := fun A B f (x : Comp A) => (v <- x; ret (f v))%comp
+}.
+
+Program Instance Comp_Applicative : Applicative Comp := {
+  pure := fun _ x => (ret x)%comp;
+  ap   := fun A B mf mx => (f <- mf; x <- mx; ret (f x))%comp
+}.
+
+Program Instance Comp_Alternative : Alternative Comp := {
+  empty  := fun A _ => False;
+  choose := fun A x y s => x s \/ y s (* jww (2016-01-28): right? *)
+}.
+
+Program Instance Comp_Monad : Monad Comp := {
+  join := fun A m => (m >>= id)%comp
+}.
+
+Module CompLaws.
+
+Require Import Here.Tactics.
+Import MonadLaws.
+
+Local Obligation Tactic := simpl; intros; simplify_comp.
+
+Program Instance Comp_FunctorLaws : FunctorLaws Comp.
+Program Instance Comp_ApplicativeLaws : ApplicativeLaws Comp.
+Program Instance Comp_MonadLaws : MonadLaws Comp.
+
+End CompLaws.
+
+Lemma ret_inj : forall A (x y : A), ret x = ret y -> x = y.
+Proof.
+  intros.
+  assert (forall P Q : Prop, P = Q -> (P <-> Q)) as Heq.
+    intros.
+    rewrite H0.
+    reflexivity.
+  pose proof (@equal_f A Prop _ _ H y) as H0.
+  apply Heq in H0.
+  destruct H0.
+  specialize (H1 (Ensembles.In_singleton A y)).
+  inversion H1.
+  reflexivity.
+Qed.
+
+Lemma refineEquiv_fmap_id {A} : refineEquiv (fmap (@id A)) id.
+Proof. reflexivity. Qed.
+
+Lemma refineEquiv_fmap_id_x {A x} : refineEquiv (fmap (@id A) x) x.
+Proof.
+  autorewrite with monad laws.
+  reflexivity.
+Qed.
+
+Lemma refineEquiv_fmap_comp {A B C} (k : B -> C) (g : A -> B) :
+  refineEquiv (fmap k \o fmap g) (fmap (k \o g)).
+Proof. reflexivity. Qed.
+
+Lemma refineEquiv_fmap_comp_x {A B C x} (k : B -> C) (g : A -> B) :
+  refineEquiv (fmap k (fmap g x)) (fmap (k \o g) x).
+Proof.
+  autorewrite with monad laws.
+  reflexivity.
+Qed.
+
+Add Parametric Morphism A B f : (@fmap Comp _ A B f)
+  with signature
+    ((@refineEquiv A) ==> (@refineEquiv B))
+  as refineEquiv_fmap.
+Proof.
+  intros x y H; simpl.
+  rewrite H.
+  reflexivity.
+Qed.
+
+Add Parametric Morphism A B : (@ap Comp _ A B)
+  with signature
+    ((@refine (A -> B)) ==> (@refine A) ==> (@refine B))
+  as refine_ap.
+Proof.
+  intros ?? H1 x y H2; simpl.
+  rewrite H1.
+  intro v; intros.
+  do 2 destruct H.
+  do 2 destruct H0.
+  destruct H3.
+  eexists.
+  split.
+    exact H.
+  eexists.
+  split.
+    rewrite H2.
+    exact H0.
+  constructor.
+Qed.
+
+Require Export Coq.Classes.Morphisms.
+Export Coq.Classes.Morphisms.ProperNotations.
+Require Export Coq.Classes.SetoidClass.
+
+(* Computations form a setoid over refinement equivalence. *)
+Program Instance Comp_Setoid : forall A, Setoid (Comp A) := {
+  equiv := refineEquiv;
+  setoid_equiv := refineEquiv_Equivalence A
+}.
+
+(* Computations and unidirectional refinement form a partial order, where the
+   ordering is a subset relation. *)
+Program Instance Comp_PreOrder : forall A, PreOrder (@refine A).
+
+(* Computations and their setoid equivalence together form a partial order. *)
+Program Instance Comp_PartialOrder :
+  forall A, PartialOrder (@refineEquiv A) (@refine A).
+Obligation 1. split; intros; apply H. Qed.
+
+(* Based on its being a partial order, we know that it's antisymmetric. *)
+Lemma Comp_Antisymmetric :
+  forall A, Antisymmetric (Comp A) (@refineEquiv A) (@refine A).
+Proof. intros; apply partial_order_antisym, Comp_PartialOrder. Qed.
+
+Notation "p ⊑ q" := (refine q p) (at level 20, only parsing).
+
+Definition galois_connection
+  {A} (p : Comp A) (RA : relation A)
+  {B} (q : Comp B) (RB : relation B)
+  (F : A -> B) (G : B -> A) :=
+    forall (a : A), p ↝ a ->
+    forall (b : B), q ↝ b ->
+    (RB (F a) b <-> RA a (G b)).
+
+Require Import ZArith.
+
+Lemma helper : forall n q, n < Z.to_nat q -> (0 < q)%Z.
+Proof.
+  intros.
+  induction n; simpl.
+  - apply Nat2Z.inj_lt in H.
+    simpl in H.
+    destruct q eqn:Heqe.
+    + inversion H.
+    + apply Pos2Z.is_pos.
+    + inversion H.
+  - apply IHn.
+    omega.
+Qed.
+
+Lemma galois : forall p q, (Z.of_nat p < q)%Z <-> p < Z.to_nat q.
+Proof.
+  intros; split; intros.
+    rewrite <- (Nat2Z.id p).
+    apply Z2Nat.inj_lt; omega.
+  rewrite <- (Nat2Z.id p) in H.
+  apply Z2Nat.inj_lt in H.
+  - assumption.
+  - omega.
+  - apply helper in H.
+    omega.
+Qed.
+
+Lemma transport_nat_Z : forall (p : Comp nat) (q : Comp Z),
+  galois_connection p lt q Z.lt Z.of_nat Z.to_nat.
+Proof.
+  unfold galois_connection; simpl; intros.
+  apply galois.
+Qed.
+
+Lemma z_to_nat_pick : forall b e, 0 <= b ->
+  refine {z : Z | (Z.of_nat b <= z < Z.of_nat e)%Z}
+         (x <- {n : nat | b <= n < e};
+          ret (Z.of_nat x)).
+Proof.
+  unfold refine; intros.
+  apply Bind_inv in H0.
+  destruct H0.
+  destruct H0.
+  apply Pick_inv in H0.
+  apply Return_inv in H1; subst.
+  destruct H0.
+  apply PickComputes.
+  split; omega.
+Qed.
+
+Ltac adjust_refine term :=
+  let T := constr:term in
+  assert { T' : _ & refine T T'} as T'; [eexists| apply (projT1 T')].
+
+Definition foo_Z : Comp Z :=
+  x <- { z : Z | (0  <= z < 10)%Z };
+  y <- { z : Z | (10 <= z < 20)%Z };
+  z <- { z : Z | (10 <= z < 20)%Z };
+  ret (x + y + z)%Z.
+
+Require Import Hask.Control.Monad.Free.
+Require Import Coq.Vectors.Vector.
+Import VectorNotations.
+
+Inductive Freeified (f : Type -> Type) (a : Type) :
+  forall (n : nat), Vector.t Type n -> Type :=
+  | Pure' : a -> Freeified f a (nil Type)
+  | Join' : forall (t : Type) (n : nat) (ts : Vector.t Type n),
+      (t -> Freeified f a ts) -> f t -> Freeified f a (cons Type t _ ts).
+
+Arguments Pure' {f a} _.
+Arguments Join' {f a _ n ts} _ _.
+
+Definition example :
+  Freeified Comp nat (cons Type Z _ (cons Type Z _ (nil Type))) :=
+  Join' (fun x : Z =>
+           Join' (fun y : Z =>
+                    Pure' (Z.to_nat (x + y)))
+                 { z : Z | z = 0%Z })
+        { z : Z | z = 0%Z }.
+
+Fixpoint retractified `{Monad f} {n} `(fr : Freeified f a (n:=n) ts) : f a :=
+  match fr with
+    | Pure' x => pure x
+    | Join' _ n ts g h => (h >>= (retractified \o g))%monad
+  end.
+
+Eval simpl in retractified example.
+
+Ltac freeify comp :=
+  match goal with
+    [ |- Freeified Comp ?T ?TS ] =>
+    assert { c : Comp T
+           & { f : Freeified Comp T TS & refineEquiv (retractified f) c } }
+      as freeified
+      by (exists comp;
+          eexists;
+          unfold comp;
+          repeat
+            match goal with
+            | [ |- refineEquiv (retractified _) (Bind ?C _) ] =>
+              instantiate (1 := Join' _ C); unfold id; simpl;
+              autorewrite with monad laws;
+              apply refineEquiv_bind; [ reflexivity |];
+              intros ?; unfold id; simpl
+            | [ |- refineEquiv (retractified (_ ?X)) (Bind ?C _) ] =>
+              instantiate (1 := fun X => Join' _ C); unfold id; simpl;
+              autorewrite with monad laws;
+              apply refineEquiv_bind; [ reflexivity |];
+              intros ?; unfold id; simpl
+            | [ |- refineEquiv (retractified _) (Return _) ] =>
+              instantiate (1 := fun _ => Pure' _); unfold id; simpl;
+              autorewrite with monad laws;
+              reflexivity
+            end);
+    exact (projT1 (projT2 freeified))
+  end.
+
+(*
+Definition foo_Z_free :
+  { n : nat & { TS : Vector.t Type n & Freeified Comp Z TS } }.
+Proof.
+  eexists.
+  eexists.
+  freeify foo_Z.
+Defined.
+
+Definition foo_Z_free' :=
+  Eval compute [foo_Z_free projT1 projT2] in projT2 (projT2 foo_Z_free).
+Print foo_Z_free'.
+*)
+
+Definition natify (f : Z -> nat) {n} {ts : Vector.t Type n}
+  (x : Freeified Comp Z (n:=n) ts) :
+  {ts' : Vector.t Type n & Freeified Comp nat (n:=n) ts'}.
+Proof.
+  induction x.
+    exists (nil Type).
+    apply Pure'.
+    exact (f a).
+Abort.
+
+(* Eval compute [natify fmap Free_Functor Free_bind foo_Z_free' comp] *)
+(*   in natify Z.to_nat foo_Z_free'. *)
+
+Example foo_nat0 : Comp nat.
+Proof.
+  adjust_refine (fmap Z.to_nat foo_Z).
+  set_evars.
+  unfold foo_Z in *; simpl.
+  unfold refine; intros.
+  eapply BindComputes.
+    eapply BindComputes.
+    evar (c : Comp nat).
+    pose proof (transport_nat_Z c {z : Z | (0 <= z < 10)%Z}).
+    unfold galois_connection in H1.
+  replace 0%Z with (Z.of_nat 0); trivial.
+  replace 10%Z with (Z.of_nat 10); trivial.
+  replace 20%Z with (Z.of_nat 20); trivial.
+  rewrite z_to_nat_pick; trivial.
+Abort.
+
+Example foo_nat0 : Comp nat.
+Proof.
+  adjust_refine (fmap Z.to_nat foo_Z).
+  unfold foo_Z; simpl.
+  replace 0%Z with (Z.of_nat 0); trivial.
+  replace 10%Z with (Z.of_nat 10); trivial.
+  replace 20%Z with (Z.of_nat 20); trivial.
+  rewrite z_to_nat_pick; trivial.
+  setoid_rewrite (z_to_nat_pick _).
+  simplify with monad laws.
+  setoid_rewrite <- Nat2Z.inj_add.
+Abort.
+
+(* Definition foo_nat0' := *)
+(*   Eval compute [foo_nat0 proj1_sig projT1] in foo_nat0. *)
+(* Print foo_nat0'. *)
+
+(*
+Example foo_nat_bad :
+  { c : Comp nat
+  | galois_inserted_if (fmap Z.of_nat) (fmap Z.to_nat)
+                       (fun z : Z => (0 <= z)%Z) c foo_Z }.
+Proof.
+  exists (ret 0).
+  unfold galois_inserted_if.
+  apply transport_nat_Z.
+Defined.
+
+Definition foo_nat_bad' :=
+  Eval compute [foo_nat_bad proj1_sig projT1] in proj1_sig foo_nat_bad.
+Print foo_nat_bad'.
+*)
+
+Example foo_nat : Comp nat.
+Proof.
+  adjust_refine (fmap Z.to_nat foo_Z).
+  unfold foo_Z; simpl.
+Abort.
+(*
+  apply transport_nat_Z; simpl.
+    intros.
+    apply Bind_inv in H.
+    do 2 destruct H.
+    apply Bind_inv in H0.
+    do 2 destruct H0.
+    apply Return_inv in H1.
+    rewrite <- H1; clear H1.
+    apply Pick_inv in H.
+    apply Pick_inv in H0.
+    abstract omega.
+  replace 0%Z with (Z.of_nat 0); trivial.
+  replace 10%Z with (Z.of_nat 10); trivial.
+  replace 20%Z with (Z.of_nat 20); trivial.
+  rewrite z_to_nat_pick; trivial.
+  setoid_rewrite (z_to_nat_pick _).
+  simplify with monad laws.
+  setoid_rewrite <- Nat2Z.inj_add.
+  assert (refineEquiv (x0 <- {n : nat | 0 <= n < 10};
+                       x1 <- {n : nat | 10 <= n < 20};
+                       ret (Z.of_nat (x0 + x1)))
+                      (v <- x0 <- {n : nat | 0 <= n < 10};
+                            x1 <- {n : nat | 10 <= n < 20};
+                            ret (x0 + x1);
+                       ret (Z.of_nat v))).
+    autorewrite with monad laws.
+    reflexivity.
+  rewrite H.
+  reflexivity.
+  Grab Existential Variables.
+  abstract omega.
+Defined.
+
+Definition foo_nat' := Eval compute [foo_nat proj1_sig projT1] in foo_nat.
+Print foo_nat'.
+*)
