src/RefinedHeap.v
@@ -43,6 +43,19 @@ Definition MemoryBlock_Same (x y : MemoryBlock) : Prop :=
 Definition MemoryBlockC_Equal (x y : MemoryBlockC) : Prop :=
   memCSize x = memCSize y /\ M.Equal (memCData x) (memCData y).
 
+Global Program Instance MemoryBlock_Proper :
+  Proper (eq ==> @Same _ _ ==> MemoryBlock_Same) (@Build_MemoryBlock Word8).
+Obligation 1. relational; split; simpl; subst; auto. Qed.
+
+Global Program Instance MemoryBlockC_Proper :
+  Proper (eq ==> @M.Equal _ ==> MemoryBlockC_Equal) Build_MemoryBlockC.
+Obligation 1. relational; split; simpl; subst; auto. Qed.
+
+Global Program Instance MemoryBlock_AbsR_AbsR :
+  (@Build_MemoryBlock Word8) [R eq ==> Map_AbsR eq ==> MemoryBlock_AbsR]
+  Build_MemoryBlockC.
+Obligation 1. relational; split; simpl; subst; auto. Qed.
+
 Global Program Instance Finite_Proper {A B} :
   Morphisms.Proper (Same (B:=B) ==> impl) (Finite (A * B)).
 Obligation 1.
@@ -255,6 +268,71 @@ Proof.
   assumption.
 Qed.
 
+Axiom Extensionality_FMap : forall (elt : Type) (A B : M.t elt),
+  M.Equal (elt:=elt) A B -> A = B.
+
+Lemma MemoryBlock_AbsR_FunctionalRelation :
+  FunctionalRelation MemoryBlock_AbsR.
+Proof.
+  intros ?????.
+  destruct H, H0, x, y, z; simpl in *.
+  subst; f_equal.
+  apply Extensionality_FMap.
+  apply F.Equal_mapsto_iff; split; intros.
+    apply H2, H1; trivial.
+  apply H1, H2; trivial.
+Qed.
+
+Hint Resolve MemoryBlock_AbsR_FunctionalRelation.
+
+Lemma MemoryBlock_AbsR_InjectiveRelation :
+  InjectiveRelation MemoryBlock_AbsR.
+Proof.
+  intros ?????.
+  destruct H, H0, x, y, z; simpl in *.
+  subst; f_equal.
+  apply Extensionality_Ensembles.
+  split; intros;
+  intros ??; destruct x.
+    apply H2, H1; trivial.
+  apply H1, H2; trivial.
+Qed.
+
+Hint Resolve MemoryBlock_AbsR_InjectiveRelation.
+
+Lemma eq_FunctionalRelation : forall A, FunctionalRelation (A:=A) (B:=A) eq.
+Proof. intros ??????; subst; reflexivity. Qed.
+
+Hint Resolve eq_FunctionalRelation.
+
+Lemma eq_InjectiveRelation : forall A,
+  InjectiveRelation (A:=A) (B:=A) eq.
+Proof. intros ??????; subst; reflexivity. Qed.
+
+Hint Resolve eq_InjectiveRelation.
+
+Lemma MemoryBlock_AbsR_TotalMapRelation :
+  forall r : Rep HeapSpec, fromADT _ r
+    -> TotalMapRelation MemoryBlock_AbsR r.
+Proof.
+  intros; intros ???.
+  pose proof (all_blocks_are_finite H _ _ H0).
+  pose proof (all_block_maps_are_unique H _ _ H0).
+  simpl in *.
+  elimtype ((exists size : N, memSize x = size) /\
+            (exists data : M.t Word8, Map_AbsR eq (memData x) data)).
+    do 2 destruct 1.
+    eexists {| memCSize := x0; memCData := x1 |}.
+    constructor; auto.
+  split; eauto.
+  apply every_finite_map_has_an_associated_fmap; auto.
+  intros ???.
+  exists x0.
+  reflexivity.
+Qed.
+
+Hint Resolve MemoryBlock_AbsR_TotalMapRelation.
+
 Theorem Peek_in_heap {r_o r_n} (AbsR : Heap_AbsR r_o r_n) pos :
   forall base blk' cblk',
     MemoryBlock_AbsR blk' cblk'
@@ -276,11 +354,9 @@ Proof.
   apply find_if_filter_is_singleton in H2.
     unfold optionP, pairP in H2.
     destruct (find_if (withinMemBlockC pos) (snd r_n)).
-      destruct p, H2; subst.
-      reflexivity.
+      destruct p, H2; subst; trivial.
     contradiction.
-  apply withinMemBlockC_Proper.
-  reflexivity.
+  apply withinMemBlockC_Proper; reflexivity.
 Qed.
 
 Theorem Poke_in_heap {r_o r_n} (AbsR : Heap_AbsR r_o r_n) pos val :
@@ -294,15 +370,14 @@ Theorem Poke_in_heap {r_o r_n} (AbsR : Heap_AbsR r_o r_n) pos val :
 Proof.
   destruct AbsR as [_ H].
   unfold P.for_all.
-  apply P.fold_rec_bis; eauto.
-  intros.
+  apply P.fold_rec_bis; auto; intros.
   apply F.mapi_mapsto_iff in H0; do 2 destruct H0;
   simpl; intros; subst; auto.
   unfold within_allocated_mem, IfDec_Then_Else; simpl.
   eapply P.for_all_iff in H; eauto.
-  unfold within_allocated_mem in H.
-  destruct ((k <=? pos) && (pos <? k + memCSize x))%bool; simpl;
-  rewrite H; assumption.
+    unfold within_allocated_mem in H.
+    destruct ((k <=? pos) && (pos <? k + memCSize x))%bool; simpl;
+    rewrite H; assumption.
   apply within_allocated_mem_Proper; reflexivity.
 Qed.
 
@@ -366,17 +441,188 @@ Proof.
   apply every_finite_map_has_an_associated_fmap; auto.
   - apply heap_is_finite; auto.
   - apply allocations_unique; auto.
-  - intros.
-    elimtype ((exists size : N, memSize e = size) /\
-              (exists data : M.t Word8, Map_AbsR eq (memData e) data)).
-      do 2 destruct 1.
-      eexists {| memCSize := x; memCData := x0 |}.
-      constructor; auto.
-    split.
-      eexists; reflexivity.
-    apply every_finite_map_has_an_associated_fmap; eauto.
-      eapply all_blocks_are_finite; eauto.
-    eapply all_block_maps_are_unique; eauto.
+Qed.
+
+Lemma find_define : forall addr len pos v w m,
+  (IfDec within addr len pos
+   Then v = w
+   Else M.MapsTo pos v m)
+    -> M.MapsTo pos v (N.peano_rect (fun _ => M.t Word8) m
+                                    (fun i => M.add (addr + i)%N w) len).
+Proof.
+  intros.
+  decisions; subst.
+    apply Bool.andb_true_iff in Heqe.
+    destruct Heqe.
+    undecide.
+    induction len using N.peano_ind; simpl in *.
+      rewrite N.add_0_r in H0.
+      nomega.
+    rewrite N.peano_rect_succ.
+    destruct (N.eq_dec pos (addr + len)); subst.
+      simplify_maps.
+      left; intuition.
+    simplify_maps.
+    right.
+    split; trivial.
+      apply not_eq_sym; assumption.
+    rewrite N.add_succ_r in H0.
+    apply N.lt_succ_r in H0.
+    pose proof (proj2 (N.le_neq pos (addr + len)) (conj H0 n)).
+    apply IHlen; assumption.
+  apply Bool.andb_false_iff in Heqe.
+  destruct Heqe; undecide;
+  induction len using N.peano_ind; simpl in *; auto;
+  rewrite N.peano_rect_succ.
+    simplify_maps.
+    right.
+    split; trivial.
+    unfold not; intros; subst.
+    rewrite <- (N.add_0_r addr) in H0 at 2.
+    apply N.add_lt_cases in H0.
+    destruct H0.
+      nomega.
+    contradiction (N.nlt_0_r len).
+  rewrite N.add_succ_r in H0.
+  simplify_maps.
+  right.
+  split.
+    unfold not; intros; subst.
+    apply N.le_succ_l in H0.
+    nomega.
+  apply IHlen.
+  apply N.le_succ_l in H0.
+  nomega.
+Qed.
+
+Lemma Nle_ne_succ : forall n m,
+  n <> m -> n < N.succ m -> n < m.
+Proof.
+  intros.
+  apply N.le_succ_l in H0.
+  apply N.succ_le_mono in H0.
+  apply N.le_neq; intuition.
+Qed.
+
+Lemma find_define_inv : forall addr len pos v w m,
+  M.MapsTo pos v (N.peano_rect (fun _ => M.t Word8) m
+                               (fun i => M.add (addr + i)%N w) len)
+    -> IfDec within addr len pos
+       Then v = w
+       Else M.MapsTo pos v m.
+Proof.
+  intros.
+  induction len using N.peano_ind; simpl in *;
+  decisions; auto.
+  - apply Bool.andb_true_iff in Heqe;
+    destruct Heqe; undecide.
+    rewrite N.add_0_r in H1.
+    nomega.
+  - rewrite N.peano_rect_succ in H.
+    simplify_maps; auto.
+  - rewrite N.peano_rect_succ in H.
+    simplify_maps; auto.
+      nomega.
+    apply Bool.andb_true_iff in Heqe;
+    destruct Heqe; undecide.
+    apply Bool.andb_false_iff in Heqe0;
+    destruct Heqe0; undecide.
+      nomega.
+    intuition; subst.
+    rewrite N.add_succ_r in H1.
+    apply N.le_succ_l in H1.
+    nomega.
+  - rewrite N.peano_rect_succ in H.
+    simplify_maps; auto.
+    intuition.
+    apply Bool.andb_true_iff in Heqe0;
+    destruct Heqe0; undecide.
+    apply Bool.andb_false_iff in Heqe;
+    destruct Heqe; undecide.
+      nomega.
+    rewrite N.add_succ_r in H1.
+    apply not_eq_sym in H3.
+    pose proof (Nle_ne_succ H3 H1).
+    nomega.
+  - rewrite N.peano_rect_succ in H.
+    simplify_maps; auto.
+    intuition.
+    apply Bool.andb_false_iff in Heqe0;
+    destruct Heqe0; undecide;
+    apply Bool.andb_false_iff in Heqe;
+    destruct Heqe; undecide.
+    + rewrite <- N.add_0_r in H0.
+      apply N.add_lt_cases in H0.
+      destruct H0.
+        nomega.
+      contradiction (N.nlt_0_r len).
+    + rewrite <- N.add_0_r in H.
+      apply N.add_lt_cases in H.
+      destruct H.
+        nomega.
+      contradiction (N.nlt_0_r len).
+    + rewrite <- N.add_0_r in H0.
+      apply N.add_lt_cases in H0.
+      destruct H0.
+        nomega.
+      contradiction (N.nlt_0_r len).
+    + rewrite N.add_succ_r in H.
+      apply N.le_succ_l in H.
+      nomega.
+Qed.
+
+Lemma Define_Map_AbsR : forall x y b len w,
+  Map_AbsR eq x y
+    -> Map_AbsR eq (Define (within b len) w x)
+                (N.peano_rect (fun _ => M.t Word8) y
+                              (fun i => M.add (b + i)%N w) len).
+Proof.
+  intros.
+  relational.
+  - teardown.
+    destruct H0, H0; [inv H1|];
+    exists blk; intuition;
+    apply find_define;
+    unfold IfDec_Then_Else; simpl.
+      apply within_reflect in H0.
+      rewrite H0; reflexivity.
+    apply not_within_reflect in H0.
+    rewrite H0.
+    apply H.
+    exists blk; intuition.
+  - reduction.
+    apply find_define_inv in H0.
+    decisions; auto; subst.
+      left.
+      apply within_reflect in Heqe.
+      intuition.
+    right.
+    apply not_within_reflect in Heqe.
+    apply H in H0.
+    destruct H0, H0; subst.
+    intuition.
+  - reduction.
+    apply find_define_inv in H0.
+    decisions; auto; subst.
+      apply within_reflect in Heqe.
+      exists w; intuition.
+      teardown.
+      left; intuition.
+    apply not_within_reflect in Heqe.
+    apply H in H0.
+    destruct H0, H0; subst.
+    exists cblk; intuition.
+    teardown.
+    right; intuition.
+  - repeat teardown; subst; [inv H2|];
+    apply find_define;
+    unfold IfDec_Then_Else; simpl.
+      apply within_reflect in H0.
+      rewrite H0; reflexivity.
+    apply not_within_reflect in H0.
+    rewrite H0.
+    apply H.
+    exists cblk; intuition.
 Qed.
 
 Lemma HeapImpl : FullySharpened HeapSpec.
@@ -478,7 +724,118 @@ Proof.
     remove_dependency.
     simplify with monad laws; simpl.
 
-    admit.
+    refine pick val
+      (match M.find d (snd r_n) with
+       | Some cblk =>
+         Some {| memSize := memCSize cblk
+               ; memData := of_map eq (memCData cblk) |}
+       | None => None
+       end).
+      Focus 2.
+      destruct (M.find (elt:=MemoryBlockC) d (snd r_n)) eqn:Heqe.
+        apply F.find_mapsto_iff, H0 in Heqe.
+        destruct Heqe, H1, H2; simpl.
+        apply of_map_Same in H3.
+        apply H0 in H1; apply H0.
+        destruct H1, H1; exists x0.
+        intuition.
+        split; intros; simpl.
+          rewrite <- (proj1 H4).
+          congruence.
+        rewrite <- H3.
+        exact (proj2 H4).
+      simpl.
+      unfold not; intros.
+      destruct H1.
+      apply H0 in H1.
+      destruct H1, H1.
+      apply F.find_mapsto_iff in H1.
+      congruence.
+
+    simplify with monad laws.
+    refine pick val
+      (Ifopt M.find d (snd r_n) as cblk
+       Then If ` d0 <? memCSize cblk
+            Then d
+            Else fst r_n
+       Else fst r_n).
+      Focus 2.
+      intros ???.
+      destruct (M.find (elt:=MemoryBlockC) d (snd r_n)) eqn:Heqe;
+      destruct d0; simpl in *;
+      decisions; undecide;
+      repeat teardown;
+      try discriminate.
+        inv Heqe.
+        reduction.
+        admit.
+      destruct H0; simpl in *.
+      apply H0 in H2.
+      do 2 destruct H2.
+      eapply P.for_all_iff with (k:=a) (e:=x1) in H3; eauto.
+        rewrite (proj1 H4).
+        unfold within_allocated_mem in H3; undecide.
+        unfold overlaps, not; intros.
+        clear -H3 H5.
+        nomega.
+      apply within_allocated_mem_Proper; auto.
+
+    simplify with monad laws.
+    refine pick val
+      (match M.find (elt:=MemoryBlockC) d (snd r_n) with
+       | Some cblk =>
+         if ` d0 <? memCSize cblk
+         then (fst r_n,
+               M.add d {| memCSize := ` d0
+                        ; memCData := P.filter (fun k e => k <? ` d0)
+                                               (memCData cblk)
+                        |} (M.remove d (snd r_n)))
+         else (* jww (2016-08-08): Next step: find a better free block *)
+              ((fst r_n + ` d0)%N,
+               M.add (fst r_n)
+                     {| memCSize := ` d0
+                      ; memCData := memCData cblk |}
+                     (M.remove d (snd r_n)))
+       | None =>
+         ((fst r_n + ` d0)%N,
+          M.add (fst r_n)
+                {| memCSize := ` d0
+                 ; memCData := M.empty _ |} (snd r_n))
+       end).
+      simplify with monad laws.
+      finish honing.
+
+    AbsR_prep.
+    - destruct (M.find (elt:=MemoryBlockC) d (snd r_n)) eqn:Heqe; simpl.
+      + decisions.
+        * admit.
+        * apply Update_Map_AbsR; auto.
+            apply MemoryBlock_AbsR_impl.
+              admit.
+            admit.
+          apply Remove_Map_AbsR; auto.
+        * apply Update_Map_AbsR; auto.
+            apply MemoryBlock_AbsR_impl; auto.
+            admit.
+          apply Remove_Map_AbsR; auto.
+        * admit.
+        * apply Update_Map_AbsR; auto.
+            apply MemoryBlock_AbsR_impl; auto.
+              admit.
+            admit.
+          apply Remove_Map_AbsR; auto.
+        * apply Update_Map_AbsR; auto.
+            apply MemoryBlock_AbsR_impl; auto.
+            admit.
+          apply Remove_Map_AbsR; auto.
+      + apply Update_Map_AbsR; auto.
+        apply MemoryBlock_AbsR_impl; auto.
+        apply Empty_Map_AbsR.
+    - destruct (M.find (elt:=MemoryBlockC) d (snd r_n)) eqn:Heqe; simpl.
+      + decisions; simpl; auto.
+        * admit.
+        * admit.
+      + admit.
   }
 
   refine method peekS.
@@ -544,7 +901,106 @@ Proof.
     remove_dependency.
     simplify with monad laws; simpl.
 
-    admit.
+    refine pick val
+      (if 0 <? d1
+       then Ifopt find_if (withinMemBlockC d) (snd r_n) as p
+            Then if Decidable_witness (P:=fits (fst p) (memCSize (snd p)) d d1)
+                 then Some (fst p,
+                            {| memSize := memCSize (snd p)
+                             ; memData := of_map eq (memCData (snd p)) |})
+                 else None
+            Else None
+       else None).
+      Focus 2.
+      intros.
+      decisions; [|discriminate].
+      undecide; intuition;
+      destruct (find_if (withinMemBlockC d) (snd r_n)) eqn:Heqe1;
+      try discriminate; simpl in H1; inv H1; simpl.
+        admit.
+      admit.
+
+    simplify with monad laws.
+    refine pick val
+      (if 0 <? d1
+       then Ifopt find_if (withinMemBlockC d0) (snd r_n) as p
+            Then if Decidable_witness (P:=fits (fst p) (memCSize (snd p)) d0 d1)
+                 then Some (fst p,
+                            {| memSize := memCSize (snd p)
+                             ; memData := of_map eq (memCData (snd p)) |})
+                 else None
+            Else None
+       else None).
+      Focus 2.
+      intros.
+      decisions; [|discriminate].
+      undecide; intuition;
+      destruct (find_if (withinMemBlockC d0) (snd r_n)) eqn:Heqe1;
+      try discriminate; simpl in H1; inv H1; simpl.
+        admit.
+      admit.
+
+    simplify with monad laws.
+    refine pick val
+      (if 0 <? d1
+       then match (find_if (withinMemBlockC d) (snd r_n),
+                   find_if (withinMemBlockC d0) (snd r_n)) with
+            | (Some (saddr, src), Some (daddr, dst)) =>
+              if (Decidable_witness
+                    (P:=fits saddr (memCSize src) d d1) &&
+                  Decidable_witness
+                    (P:=fits daddr (memCSize dst) d0 d1))%bool
+              then (fst r_n,
+                    let soff := d - saddr in
+                    let doff := d0 - daddr in
+                    M.add d0 {| memCSize := memCSize dst
+                              ; memCData :=
+                                  let d :=
+                                      P.filter (fun k _ =>
+                                                  Decidable_witness
+                                                    (P:=~ within doff d1 k))
+                                               (memCData dst) in
+                                  let s :=
+                                      P.filter (fun k _ =>
+                                                  Decidable_witness
+                                                    (P:=~ within soff d1 k))
+                                               (memCData src) in
+                                  P.update d s |}
+                          (M.remove d0 (snd r_n)))
+              else r_n
+            | _ => r_n
+            end
+       else r_n).
+      simplify with monad laws.
+      finish honing.
+
+    AbsR_prep.
+    - destruct (0 <? d1); simpl; auto.
+      destruct (find_if (withinMemBlockC d) (snd r_n)) eqn:Heqe1;
+      destruct (find_if (withinMemBlockC d0) (snd r_n)) eqn:Heqe2;
+      simpl; auto;
+      decisions; simpl; auto;
+      try destruct p;
+      try destruct p0; simpl in *;
+      decisions; simpl; auto.
+      + apply Update_Map_AbsR; auto.
+        * admit.
+        * apply MemoryBlock_AbsR_impl; auto.
+          (* apply Union_Map_AbsR; auto. *)
+          admit.
+        * admit.
+      + admit.
+      + admit.
+      + admit.
+    - destruct (0 <? d1); simpl; auto;
+      destruct (find_if (withinMemBlockC d) (snd r_n)) eqn:Heqe1;
+      destruct (find_if (withinMemBlockC d0) (snd r_n)) eqn:Heqe2;
+      simpl; auto;
+      decisions; simpl; auto;
+      try destruct p;
+      try destruct p0; simpl in *;
+      decisions; simpl; auto.
+      admit.
   }
 
   refine method memsetS.
@@ -553,7 +1009,36 @@ Proof.
     remove_dependency.
     simplify with monad laws; simpl.
 
-    admit.
+    refine pick val
+      (fst r_n,
+       M.mapi (fun addr cblk =>
+                 IfDec fits addr (memCSize cblk) d d0
+                 Then {| memCSize := memCSize cblk
+                       ; memCData :=
+                           let base := d - addr in
+                           N.peano_rect (fun _ => M.t Word8)
+                                        (memCData cblk)
+                                        (fun i => M.add (base + i)%N d1) d0  |}
+                 Else cblk) (snd r_n)).
+      simplify with monad laws.
+      finish honing.
+
+    AbsR_prep.
+    - apply Map_Map_AbsR; auto;
+      relational; subst; auto.
+      destruct x0, y0, H3; simpl in *; subst.
+      eapply MemoryBlock_AbsR_impl; eauto;
+      decisions; auto.
+      apply Define_Map_AbsR; auto.
+    - eapply P.for_all_iff.
+      + apply within_allocated_mem_Proper; auto.
+      + intros.
+        do 2 simplify_maps; subst.
+        apply P.for_all_iff with (k:=k) (e:=cblk) in H1; auto.
+        decisions; auto.
+        * apply within_allocated_mem_Proper; auto.
+        * intros; subst; reflexivity.
+        * intros; subst; reflexivity.
   }
 
   finish_SharpeningADT_WithoutDelegation.
