src/Tactics.v
@@ -60,3 +60,92 @@ Tactic Notation "refine" "method" constr(name) :=
     | _ =>
       fail "Incorrect method name"
   end.
+
+Require Import
+  Coq.Sets.Ensembles
+  Fiat.ADT
+  Fiat.ADTNotation
+  Hask.Ltac
+  FunctionalExtensionality.
+
+Axiom prop_ext : forall (P Q : Prop), (P <-> Q) -> P = Q.
+
+Ltac shatter :=
+  unfold comp, id in *;
+  repeat
+    match goal with
+    | [ H : and _ _            |- _                 ] => destruct H
+    | [ H : Bind _ _ _         |- _                 ] => destruct H
+    | [ H : In _ _ _           |- _                 ] => destruct H
+    | [ H : Datatypes.prod _ _ |- _                 ] => destruct H
+    | [                        |- and _ _           ] => split
+    | [                        |- Bind _ _ _        ] => eexists
+    | [                        |- In _ _ _          ] => constructor
+    | [                        |- In _ _ _          ] => solve [ eauto ]
+    | [                        |- In _ (Bind _ _) _ ] => eexists
+    | [                        |- In _ _ _          ] => econstructor
+    end;
+  simpl in *.
+
+(** jww (2016-04-05): Until the FunctorLaws are expressed in terms of some
+    arbitrary equivalence, we need to use functional and propositional
+    extensionality. *)
+
+Ltac simplify_comp :=
+  repeat let x := fresh "x" in extensionality x;
+  try (apply prop_ext; split; intros);
+  repeat shatter;
+  try constructor; eauto.
+
+Ltac zoom T :=
+  let Ty := type of T in
+  let U := fresh "U" in evar (U : Ty);
+  let H := fresh "H" in assert (T = U) as H;
+    [ subst U | setoid_rewrite H; clear H; unfold U; clear U ].
+
+Ltac shift tac := etransitivity; [apply tac|].
+
+Lemma surjective_pairing_r : forall A B (x : A * B),
+  (fst x, snd x) = x.
+Proof.
+  intros.
+  destruct x; reflexivity.
+Qed.
+
+Ltac adjust term :=
+  let T := constr:term in
+  assert { T' : _ & T = T'} as T'; [eexists| apply (projT1 T')].
+
+Require Import
+  Fiat.ADTRefinement
+  Fiat.ADTRefinement.BuildADTRefinements.
+
+Tactic Notation "refine" "method" constr(name) :=
+  match goal with
+    | [ _ : constructorType ?A (consDom {| consID := name
+                                         ; consDom := _ |}) |- _ ] =>
+      idtac "Constructor"
+    | [ _ : methodType ?A (methDom {| methID := name
+                                    ; methDom := _
+                                    ; methCod := _ |})  _ |- _ ] =>
+      idtac "Method"
+    | _ =>
+      fail "Incorrect method name"
+  end.
+
+Ltac finish_concrete :=
+  match goal with
+  | [ |- context[Pick _] ] => idtac
+  | _ => finish honing
+  end.
+
+Ltac simplify_ADT :=
+  try simplify with monad laws; simpl;
+  try match goal with
+    [ H : _ = _ |- _ ] =>
+    rewrite H; clear H
+  end;
+  try refine pick eq;
+  try refine pick val tt; try tauto;
+  try simplify with monad laws;
+  try finish_concrete.
